Fix circular dependencies.

rust/implementation/openssl3_impl/tunnel/mod.rs
@@ -3,8 +3,7 @@
 
 //! Tunnel implementation using OpenSSL 3 and oqs-provider.
 
-use bio_method::BIO_METHOD;
-use ssl::{Ssl, TunnelBuilder};
+// use bio_method::BIO_METHOD;
 use verify_callback::verify_callback;
 use x509_verify_param::X509VerifyParam;
 use crate::support::Pimpl;
@@ -52,4 +51,2287 @@ pub struct Context<'a> {
 
     /// Execution mode.
     mode: Mode,
+}
+
+// ######### Inlining ssl.rs ############ ///
+
+// Copyright (c) SandboxAQ. All rights reserved.
+// SPDX-License-Identifier: AGPL-3.0-only
+
+// Wrapper around the SSL object for OpenSSL 3 tunnels.
+
+use std::ffi::{c_int, c_void, CString};
+use std::pin::Pin;
+use std::ptr::NonNull;
+
+use crate::tunnel::tls::VerifierSanitizer;
+use crate::Result;
+
+use crate::ossl3::{Error, ErrorLibrary, SslError};
+
+use crate::ossl3::NativeBio;
+
+/// Index in the SSL user data (`SSL_get_ex_data`/`SSL_set_ex_data`) where
+/// the pointer to the tunnel security requirements is stored.
+const SSL_EX_DATA_TUNNEL_SECURITY_REQUIREMENTS_INDEX: c_int = 1;
+
+/// Wrapper of the OpenSSL SSL object.
+pub(super) struct Ssl(NonNull<NativeSsl>);
+
+impl std::fmt::Debug for Ssl {
+    fn fmt(&self, f: &mut std::fmt::Formatter) -> std::fmt::Result {
+        write!(f, "OpenSSL3SSLObject({:p})", self.0)
+    }
+}
+
+impl From<NonNull<NativeSsl>> for Ssl {
+    fn from(ssl: NonNull<NativeSsl>) -> Self {
+        Self(ssl)
+    }
+}
+
+impl Ssl {
+    /// Returns a pointer to some extra data from a SSL object.
+    fn get_extra_data_ptr<T>(&self, extra_data_index: impl Into<c_int>) -> Option<NonNull<T>> {
+        NonNull::new(
+            unsafe { openssl3::SSL_get_ex_data(self.0.as_ptr(), extra_data_index.into()) }
+                .cast::<T>(),
+        )
+    }
+
+    /// Returns a reference to some extra data from a SSL object.
+    fn get_extra_data_ref<'a, T>(&self, extra_data_index: impl Into<c_int>) -> Option<&'a T> {
+        self.get_extra_data_ptr::<T>(extra_data_index)
+            .map(|ptr| unsafe { ptr.as_ref() })
+    }
+
+    /// Returns the last recorded error.
+    fn get_last_recorded_error(
+        &self,
+        ret: impl Into<c_int>,
+    ) -> std::result::Result<SslError, c_int> {
+        let err = unsafe { openssl3::SSL_get_error(self.0.as_ref(), ret.into()) };
+        SslError::try_from(err).map_err(|_| err)
+    }
+
+    /// Returns the tunnel security requirements from a SSL object.
+    pub(super) fn get_tunnel_security_requirements<'a>(
+        &self,
+    ) -> Option<&'a tls::TunnelSecurityRequirements> {
+        self.get_extra_data_ref::<tls::TunnelSecurityRequirements>(
+            SSL_EX_DATA_TUNNEL_SECURITY_REQUIREMENTS_INDEX,
+        )
+    }
+
+    /// Sets the required Subject Alternative Names (SAN) specified in the [`pb_api::TunnelVerifier`]
+    /// object.
+    fn set_subject_alternative_names(
+        &self,
+        tunnel_verifier: Option<&pb_api::TunnelVerifier>,
+    ) -> Result<()> {
+        let Some(pb_api::verifiers::tunnel_verifier::Verifier::SanVerifier(san_verifier)) =
+            tunnel_verifier.and_then(|tv| tv.verifier.as_ref())
+        else {
+            return Ok(());
+        };
+        let x509_verify_param = X509VerifyParam::try_from(self.0)?;
+        for san in san_verifier.alt_names.iter() {
+            let Some(san) = san.san.as_ref() else {
+                return Err((pb::TunnelError::TUNNELERROR_VERIFIER, "empty SANMatcher").into());
+            };
+            x509_verify_param.add_san(san)?;
+        }
+        Ok(())
+    }
+
+    /// Sets the server name indication (SNI).
+    fn set_server_name_indication(&self, sni: impl AsRef<str>) -> Result<()> {
+        let sni = sni.as_ref();
+        if sni.is_empty() {
+            return Ok(());
+        }
+        let cstring = CString::new(sni).map_err(|e| {
+            (
+                pb::SystemError::SYSTEMERROR_MEMORY,
+                format!("failed to create a c-string for the SNI '{sni}': {e}"),
+            )
+        })?;
+        // `SSL_set_tlsext_host_name` is a C macro.
+        if unsafe {
+            openssl3::SSL_ctrl(
+                self.0.as_ptr(),
+                openssl3::SSL_CTRL_SET_TLSEXT_HOSTNAME as c_int,
+                openssl3::TLSEXT_NAMETYPE_host_name as i64,
+                cstring.as_ptr().cast::<c_void>().cast_mut(),
+            )
+        } == 1
+        {
+            Ok(())
+        } else {
+            Err((
+                pb::TunnelError::TUNNELERROR_VERIFIER,
+                format!("failed to set the SNI to '{sni}': {}", crate::ossl3::errstr()),
+            )
+                .into())
+        }
+    }
+
+    /// Creates a new Sandwich BIO and attach it to the SSL object.
+    fn create_and_attach_bio(&self) -> Result<()> {
+        let bio = crate::ossl3::new_BIO(BIO_METHOD)?;
+        let ptr = bio.as_nonnull().as_ptr();
+        unsafe {
+            openssl3::BIO_set_init(ptr, 1);
+            openssl3::SSL_set_bio(self.0.as_ptr(), ptr, ptr);
+        }
+        let _ = bio.into_raw();
+        Ok(())
+    }
+
+    /// Returns a pointer to the BIO currently attached to the SSL object.
+    fn get_attached_bio(&self) -> Option<NonNull<NativeBio>> {
+        NonNull::new(unsafe { openssl3::SSL_get_rbio(self.0.as_ptr()) })
+    }
+
+    /// Returns the state of the SSL tunnel.
+    fn get_state(&self) -> pb::HandshakeState {
+        if unsafe { openssl3::SSL_get_state(self.0.as_ptr()) }
+            == openssl3::OSSL_HANDSHAKE_STATE_TLS_ST_OK
+        {
+            pb::HandshakeState::HANDSHAKESTATE_DONE
+        } else {
+            pb::HandshakeState::HANDSHAKESTATE_IN_PROGRESS
+        }
+    }
+
+    /// Checks if the tunnel is in a shutdown state.
+    fn is_shutdown(&self) -> bool {
+        let shutdown_state = unsafe { openssl3::SSL_get_shutdown(self.0.as_ptr()) } as u32;
+        (shutdown_state & (openssl3::SSL_SENT_SHUTDOWN | openssl3::SSL_RECEIVED_SHUTDOWN)) != 0
+    }
+
+    /// Performs the handshake.
+    fn do_handshake(&self) -> (Result<pb::HandshakeState>, Option<pb::State>) {
+        let handshake_error = unsafe { openssl3::SSL_do_handshake(self.0.as_ptr()) };
+
+        if handshake_error == 1 {
+            return (
+                Ok(pb::HandshakeState::HANDSHAKESTATE_DONE),
+                Some(pb::State::STATE_HANDSHAKE_DONE),
+            );
+        }
+        let ssl_error = match self.get_last_recorded_error(handshake_error) {
+            Ok(ssl_error) => ssl_error,
+            Err(error_code) => {
+                return (
+                    Err((
+                        pb::HandshakeError::HANDSHAKEERROR_UNKNOWN_ERROR,
+                        format!(
+                            "unexpected `SSL_ERROR_SSL` (code {error_code}) from OpenSSL: {}",
+                            crate::ossl3::errstr()
+                        ),
+                    )
+                        .into()),
+                    None,
+                );
+            }
+        };
+
+        match ssl_error {
+            SslError::WantRead => (
+                Ok(pb::HandshakeState::HANDSHAKESTATE_WANT_READ),
+                Some(pb::State::STATE_HANDSHAKE_IN_PROGRESS),
+            ),
+            SslError::WantWrite => (
+                Ok(pb::HandshakeState::HANDSHAKESTATE_WANT_WRITE),
+                Some(pb::State::STATE_HANDSHAKE_IN_PROGRESS),
+            ),
+            SslError::ZeroReturn => (
+                Ok(pb::HandshakeState::HANDSHAKESTATE_IN_PROGRESS),
+                Some(pb::State::STATE_HANDSHAKE_IN_PROGRESS),
+            ),
+            SslError::WantAccept | SslError::WantConnect => (
+                Ok(pb::HandshakeState::HANDSHAKESTATE_IN_PROGRESS),
+                Some(pb::State::STATE_NOT_CONNECTED),
+            ),
+            SslError::Ssl => self.handle_ssl_error_ssl(),
+            _ => (
+                Err((
+                    pb::HandshakeError::HANDSHAKEERROR_UNKNOWN_ERROR,
+                    format!(
+                        "unexpected SSL error from OpenSSL: {ssl_error:?} ({})",
+                        crate::ossl3::errstr()
+                    ),
+                )
+                    .into()),
+                None,
+            ),
+        }
+    }
+
+    /// Reads some data and writes it to a buffer.
+    fn read(&self, buffer: &mut [u8]) -> crate::tunnel::RecordResult<usize> {
+        let buf_len: i32 = buffer
+            .len()
+            .try_into()
+            .map_err(|_| pb::RecordError::RECORDERROR_TOO_BIG)?;
+
+        let err =
+            unsafe { openssl3::SSL_read(self.0.as_ptr(), buffer.as_mut_ptr().cast(), buf_len) };
+        if err > 0 {
+            return Ok(err as usize);
+        }
+        Err(self.get_error_from_record_stage(err).into())
+    }
+
+    /// Write some data.
+    fn write(&self, buffer: &[u8]) -> crate::tunnel::RecordResult<usize> {
+        let buf_len: i32 = buffer
+            .len()
+            .try_into()
+            .map_err(|_| pb::RecordError::RECORDERROR_TOO_BIG)?;
+
+        let err = unsafe { openssl3::SSL_write(self.0.as_ptr(), buffer.as_ptr().cast(), buf_len) };
+        if err > 0 {
+            return Ok(err as usize);
+        }
+        Err(self.get_error_from_record_stage(err).into())
+    }
+
+    /// Returns the error that occurred during the record stage.
+    ///
+    /// The record stage is the stage when `SSL_read` and `SSL_write`
+    /// are called.
+    fn get_error_from_record_stage(&self, err: c_int) -> pb::RecordError {
+        let Ok(ssl_error) = self.get_last_recorded_error(err) else {
+            return pb::RecordError::RECORDERROR_UNKNOWN;
+        };
+        if (ssl_error == SslError::Syscall) && (err == 0) {
+            return pb::RecordError::RECORDERROR_CLOSED;
+        }
+        ssl_error.into()
+    }
+
+    /// Closes the tunnel.
+    fn close(&self) -> crate::tunnel::RecordResult<()> {
+        unsafe { openssl3::SSL_shutdown(self.0.as_ptr()) };
+        Ok(())
+    }
+
+    /// Handles an SSL error of type `SSL_ERROR_SSL`.
+    fn handle_ssl_error_ssl(&self) -> (Result<pb::HandshakeState>, Option<pb::State>) {
+        let error = Error::from(crate::ossl3::peek_last_error());
+
+        if error.library() != ErrorLibrary::Ssl {
+            return (
+                Err((
+                    pb::HandshakeError::HANDSHAKEERROR_UNKNOWN_ERROR,
+                    format!(
+                        "unexpected error from OpenSSL: {error:?} ({})",
+                        crate::ossl3::errstr()
+                    ),
+                )
+                    .into()),
+                None,
+            );
+        }
+        match error.reason() {
+            openssl3::SSL_R_UNSUPPORTED_PROTOCOL => {
+                return (
+                    Err((
+                        pb::HandshakeError::HANDSHAKEERROR_UNSUPPORTED_PROTOCOL,
+                        format!(
+                            "unsupported TLS protocol. error: {error:?} ({})",
+                            crate::ossl3::errstr()
+                        ),
+                    )
+                        .into()),
+                    None,
+                );
+            }
+            openssl3::SSL_R_NO_SHARED_CIPHER => {
+                return (
+                    Err((
+                        pb::HandshakeError::HANDSHAKEERROR_NO_SHARED_CIPHER,
+                        format!("no shared cipher. error: {error:?} ({})", crate::ossl3::errstr()),
+                    )
+                        .into()),
+                    None,
+                );
+            }
+            openssl3::SSL_R_NO_SUITABLE_KEY_SHARE => {
+                return (
+                    Err((
+                        pb::HandshakeError::HANDSHAKEERROR_NO_SUITABLE_KEY_SHARE,
+                        format!(
+                            "no suitable key share found. error: {error:?} ({})",
+                            crate::ossl3::errstr()
+                        ),
+                    )
+                        .into()),
+                    None,
+                );
+            }
+            openssl3::SSL_R_CERTIFICATE_VERIFY_FAILED => {}
+            _ => {
+                return (
+                    Err((
+                        pb::HandshakeError::HANDSHAKEERROR_UNKNOWN_ERROR,
+                        format!(
+                            "unexpected SSL error from OpenSSL: {error:?} ({})",
+                            crate::ossl3::errstr()
+                        ),
+                    )
+                        .into()),
+                    None,
+                );
+            }
+        }
+
+        let verify_result = unsafe { openssl3::SSL_get_verify_result(self.0.as_ptr()) } as u32;
+        let err: crate::Error = match verify_result {
+            openssl3::X509_V_ERR_CERT_HAS_EXPIRED => {
+                pb::HandshakeError::HANDSHAKEERROR_CERTIFICATE_EXPIRED.into()
+            }
+            openssl3::X509_V_ERR_CERT_REVOKED => {
+                pb::HandshakeError::HANDSHAKEERROR_CERTIFICATE_REVOKED.into()
+            }
+            openssl3::X509_V_ERR_CERT_SIGNATURE_FAILURE => {
+                pb::HandshakeError::HANDSHAKEERROR_CERTIFICATE_SIGNATURE_VERIFICATION_FAILED.into()
+            }
+            openssl3::X509_V_ERR_CA_CERT_MISSING_KEY_USAGE => {
+                pb::HandshakeError::HANDSHAKEERROR_CERTIFICATE_VERIFICATION_FAILED.into()
+            }
+            openssl3::X509_V_ERR_HOSTNAME_MISMATCH => (
+                pb::HandshakeError::HANDSHAKEERROR_INVALID_SERVER_NAME,
+                "hostname mismatches",
+            )
+                .into(),
+            openssl3::X509_V_ERR_EMAIL_MISMATCH => (
+                pb::HandshakeError::HANDSHAKEERROR_INVALID_SERVER_NAME,
+                "email mismatches",
+            )
+                .into(),
+            openssl3::X509_V_ERR_IP_ADDRESS_MISMATCH => (
+                pb::HandshakeError::HANDSHAKEERROR_INVALID_SERVER_NAME,
+                "ip address mismatches",
+            )
+                .into(),
+            openssl3::X509_V_ERR_CERT_CHAIN_TOO_LONG => {
+                pb::HandshakeError::HANDSHAKEERROR_DEPTH_EXCEEDED.into()
+            }
+            openssl3::X509_V_ERR_CERT_NOT_YET_VALID
+            | openssl3::X509_V_ERR_CERT_UNTRUSTED
+            | openssl3::X509_V_ERR_CERT_REJECTED => (
+                pb::HandshakeError::HANDSHAKEERROR_INVALID_CERTIFICATE,
+                "certificate not yet valid, untrusted or rejected",
+            )
+                .into(),
+            _ => (
+                pb::HandshakeError::HANDSHAKEERROR_UNKNOWN_ERROR,
+                format!(
+                    "verification failed: verify code is {verify_result}, error: {}",
+                    crate::ossl3::errstr()
+                ),
+            )
+                .into(),
+        };
+        (Err(err), None)
+    }
+}
+
+/// Verifies the tunnel configuration against the security requirements that come
+/// from the context.
+fn verify_tunnel_verifier(
+    tunnel_verifier: Option<&pb_api::TunnelVerifier>,
+    security_requirements: &tls::TunnelSecurityRequirements,
+) -> Result<()> {
+    let Some(tunnel_verifier) = tunnel_verifier else {
+        return Err((pb::TunnelError::TUNNELERROR_VERIFIER, "empty verifier").into());
+    };
+
+    security_requirements.run_sanitizer_checks(tunnel_verifier)
+}
+
+impl std::fmt::Debug for Tunnel<'_> {
+    fn fmt(&self, f: &mut std::fmt::Formatter) -> std::fmt::Result {
+        write!(
+            f,
+            "OpenSSL3Tunnel(ssl: {:p})",
+            self.ssl.as_nonnull().as_ptr()
+        )
+    }
+}
+
+/// Tunnel builder.
+/// This is a convenient aggregate of useful values to build a tunnel.
+pub(crate) struct TunnelBuilder<'a> {
+    /// Parent SSL_CTX object.
+    pub(crate) ssl_ctx: &'a Context<'a>,
+
+    /// The IO interface.
+    pub(crate) io: BoxedIO,
+
+    /// The tunnel-time configuration.
+    pub(crate) configuration: pb_api::TunnelConfiguration,
+}
+
+/// Tunnel builder result.
+type TunnelBuilderResult<'a> =
+    std::result::Result<Pin<Box<Tunnel<'a>>>, (crate::Error, BoxedIO)>;
+
+impl std::fmt::Debug for TunnelBuilder<'_> {
+    fn fmt(&self, f: &mut std::fmt::Formatter) -> std::fmt::Result {
+        write!(f, "OpenSSL3TunnelBuilder")
+    }
+}
+
+impl<'a> TunnelBuilder<'a> {
+    /// Prepares a tunnel structure.
+    fn prepare_ssl(&self) -> Result<Pimpl<'a, NativeSsl>> {
+        let tunnel_verifier = self.configuration.verifier.as_ref();
+        let security_requirements = self.ssl_ctx.security_requirements();
+        verify_tunnel_verifier(tunnel_verifier, security_requirements)?;
+
+        let ssl = self.ssl_ctx.new_ssl()?;
+        let ssl_wrapped = Ssl(ssl.as_nonnull());
+        ssl_wrapped.set_subject_alternative_names(tunnel_verifier)?;
+        ssl_wrapped.set_server_name_indication(&self.configuration.server_name_indication)?;
+        ssl_wrapped.create_and_attach_bio()?;
+        Ok(ssl)
+    }
+
+    /// Builds a tunnel.
+    pub(crate) fn build(self) -> TunnelBuilderResult<'a> {
+        let ssl = match self.prepare_ssl() {
+            Ok(ssl) => ssl,
+            Err(e) => {
+                return Err((e, self.io));
+            }
+        };
+        let tun = Box::pin(Tunnel {
+            _ssl_ctx: self.ssl_ctx,
+            ssl,
+            io: self.io,
+            security_requirements: self.ssl_ctx.security_requirements().clone(),
+            state: pb::State::STATE_NOT_CONNECTED,
+        });
+        if let Err(e) = tun.as_ref().attach_security_requirements() {
+            return Err((e, unsafe { Pin::into_inner_unchecked(tun) }.io));
+        }
+        if let Err(e) = tun.as_ref().attach_to_bio() {
+            return Err((e, unsafe { Pin::into_inner_unchecked(tun) }.io));
+        }
+        Ok(tun)
+    }
+}
+
+impl<'a> Tunnel<'a> {
+    /// Attaches the security requirements structure to the `SSL` object
+    /// through `ex_data`.
+    fn attach_security_requirements(self: Pin<&Self>) -> Result<()> {
+        if unsafe {
+            openssl3::SSL_set_ex_data(
+                self.ssl.as_nonnull().as_ptr(),
+                SSL_EX_DATA_TUNNEL_SECURITY_REQUIREMENTS_INDEX,
+                (&self.security_requirements as *const tls::TunnelSecurityRequirements
+                    as *const c_void)
+                    .cast_mut(),
+            )
+        } == 1
+        {
+            Ok(())
+        } else {
+            Err((
+                pb::SystemError::SYSTEMERROR_BACKEND,
+                format!("`SSL_set_ex_data` failed: {}", crate::ossl3::errstr()),
+            )
+                .into())
+        }
+    }
+
+    /// Attaches itself to the current BIO.
+    fn attach_to_bio(self: Pin<&Self>) -> Result<()> {
+        let bio = Ssl(self.ssl.as_nonnull()).get_attached_bio().ok_or((
+            pb::SystemError::SYSTEMERROR_BACKEND,
+            "no BIO attached to the current SSL object",
+        ))?;
+        unsafe {
+            openssl3::BIO_set_data(
+                bio.as_ptr(),
+                (self.get_ref() as *const Self as *const c_void).cast_mut(),
+            )
+        };
+        Ok(())
+    }
+
+    /// Updates the state of the tunnel.
+    /// This method must be called after any read or write operation.
+    fn update_state(&mut self) {
+        if Ssl(self.ssl.as_nonnull()).is_shutdown() {
+            self.state = pb::State::STATE_DISCONNECTED;
+        }
+    }
+
+    pub(crate) fn state(&self) -> crate::tunnel::State {
+        self.state.into()
+    }
+
+    pub(crate) fn handshake(mut self) -> (Self, Result<crate::tunnel::HandshakeState>) {
+        if self.state == pb::State::STATE_HANDSHAKE_DONE {
+            return (self, Ok(pb::HandshakeState::HANDSHAKESTATE_DONE.into()));
+        }
+
+        let ssl_wrapped = Ssl(self.ssl.as_nonnull());
+
+        let state = ssl_wrapped.get_state();
+        if state == pb::HandshakeState::HANDSHAKESTATE_DONE {
+            self.state = pb::State::STATE_HANDSHAKE_DONE;
+            return (self, Ok(state.into()));
+        }
+
+        let (handshake_state, tunnel_state) = ssl_wrapped.do_handshake();
+        if let Some(tunnel_state) = tunnel_state {
+            self.state = tunnel_state;
+        }
+        (self, handshake_state.map(crate::tunnel::HandshakeState::from))
+    }
+
+    pub(crate) fn read(mut self, buf: &mut [u8]) -> (Self, crate::tunnel::RecordResult<usize>) {
+        let result = Ssl(self.ssl.as_nonnull()).read(buf);
+        self.update_state();
+        if self.state == pb::State::STATE_DISCONNECTED {
+            (self, Err(pb::RecordError::RECORDERROR_CLOSED.into()))
+        } else {
+            (self, result)
+        }
+    }
+
+    pub(crate) fn write(mut self, buf: &[u8]) -> (Self, crate::tunnel::RecordResult<usize>) {
+        let result = Ssl(self.ssl.as_nonnull()).write(buf);
+        self.update_state();
+        if self.state == pb::State::STATE_DISCONNECTED {
+            (self, Err(pb::RecordError::RECORDERROR_CLOSED.into()))
+        } else {
+            (self, result)
+        }
+    }
+
+    #[cfg(feature = "tracer")]
+    pub(crate) fn add_tracer(self, _tracer: crate::support::tracing::SandwichTracer) -> Self {
+        unimplemented!("tracing is not supported with OpenSSL 3");
+    }
+
+    pub(crate) fn close(mut self) -> (Self, crate::tunnel::RecordResult<()>) {
+        if self.state == pb::State::STATE_DISCONNECTED {
+            return (self, Ok(()));
+        }
+        let result = Ssl(self.ssl.as_nonnull()).close();
+        self.update_state();
+        if self.state == pb::State::STATE_DISCONNECTED {
+            (self, Ok(()))
+        } else {
+            (self, result)
+        }
+    }
+}
+
+#[cfg(test)]
+mod test {
+    use super::*;
+
+    /// Tests [`verify_tunnel_verifier`].
+    #[test]
+    fn test_verify_tunnel_verifier() {
+        let security_requirements = tls::TunnelSecurityRequirements {
+            allow_expired_certificate: false,
+        };
+        let tunnel_verifier = protobuf::text_format::parse_from_str(
+            r#"
+                san_verifier <
+                    alt_names <
+                        dns: "example.com"
+                    >
+                    alt_names <
+                        email: "user@example.com"
+                    >
+                    alt_names <
+                        ip_address: "127.0.0.1"
+                    >
+                >
+            "#,
+        )
+        .unwrap();
+
+        let result = verify_tunnel_verifier(Some(&tunnel_verifier), &security_requirements);
+
+        result.expect("`verify_tunnel_verifier` failed");
+    }
+
+    /// Tests [`verify_tunnel_verifier`] with no specified verifier.
+    #[test]
+    fn test_verify_tunnel_verifier_none() {
+        let security_requirements = tls::TunnelSecurityRequirements {
+            allow_expired_certificate: false,
+        };
+        let tunnel_verifier = protobuf::text_format::parse_from_str("").unwrap();
+
+        let result = verify_tunnel_verifier(Some(&tunnel_verifier), &security_requirements);
+
+        result.expect_err("`verify_tunnel_verifier` succeed");
+    }
+
+    /// Tests [`verify_tunnel_verifier`] with an empty verifier.
+    #[test]
+    fn test_verify_tunnel_verifier_empty() {
+        let security_requirements = tls::TunnelSecurityRequirements {
+            allow_expired_certificate: false,
+        };
+        let tunnel_verifier = protobuf::text_format::parse_from_str("empty_verifier<>").unwrap();
+
+        let result = verify_tunnel_verifier(Some(&tunnel_verifier), &security_requirements);
+
+        result.expect("`verify_tunnel_verifier` failed");
+    }
+}
+
+// ######### Inlining context.rs ############ ///
+// Copyright (c) SandboxAQ. All rights reserved.
+// SPDX-License-Identifier: AGPL-3.0-only
+
+// Tunnel implementation usiong OpenSSL 3 and oqs-provider.
+
+use std::borrow::Borrow;
+use std::ptr;
+
+use crate::tunnel::tls::{TlsVersion, VerifyMode};
+
+use crate::ossl3::{NativePrivateKey, NativeX509Certificate};
+
+impl std::fmt::Debug for Context<'_> {
+    fn fmt(&self, f: &mut std::fmt::Formatter) -> std::fmt::Result {
+        write!(f, "OpenSSL3Context(mode={mode:?})", mode = self.mode)
+    }
+}
+
+impl Borrow<tls::TunnelSecurityRequirements> for Context<'_> {
+    fn borrow(&self) -> &tls::TunnelSecurityRequirements {
+        &self.security_requirements
+    }
+}
+
+/// Instantiates a new SSL context (`SSL_CTX`).
+fn new_ssl_context<'a, 'b>(lib_ctx: &'a LibCtx<'static>, mode: Mode) -> Result<Pimpl<'b, NativeSslCtx>>
+where
+    'a: 'b,
+{
+    unsafe {
+        Pimpl::new(
+            openssl3::SSL_CTX_new_ex(
+                lib_ctx.as_nonnull().as_ptr(),
+                ptr::null(),
+                match mode {
+                    Mode::Client => openssl3::TLS_client_method(),
+                    Mode::Server => openssl3::TLS_server_method(),
+                },
+            ),
+            |ptr| openssl3::SSL_CTX_free(ptr),
+        )
+    }
+    .ok_or_else(|| {
+        (
+            pb::SystemError::SYSTEMERROR_MEMORY,
+            "failed to instantiate a new `SSL_CTX`",
+        )
+            .into()
+    })
+}
+
+/// Converts a [`TlsVersion`] into the corresponding OpenSSL symbol.
+impl From<TlsVersion> for i64 {
+    fn from(tls_version: TlsVersion) -> Self {
+        match tls_version {
+            TlsVersion::Tls12 => openssl3::TLS1_2_VERSION,
+            TlsVersion::Tls13 => openssl3::TLS1_3_VERSION,
+        }
+        .into()
+    }
+}
+
+/// Convenient wrapper around a `SSL_CTX`.
+struct SslContext(NonNull<NativeSslCtx>);
+
+impl std::fmt::Debug for SslContext {
+    fn fmt(&self, f: &mut std::fmt::Formatter) -> std::fmt::Result {
+        write!(f, "SslContext({:p})", self.0.as_ptr())
+    }
+}
+
+impl SslContext {
+    /// Disables session caching on a SSL context.
+    fn disable_session_cache_mode(&self) {
+        // `SSL_CTX_set_session_cache_mode` is a C macro.
+        unsafe {
+            openssl3::SSL_CTX_ctrl(
+                self.0.as_ptr(),
+                openssl3::SSL_CTRL_SET_SESS_CACHE_MODE as i32,
+                openssl3::SSL_SESS_CACHE_OFF.into(),
+                ptr::null_mut(),
+            )
+        };
+    }
+
+    /// Defines the minimum TLS version to use.
+    fn set_minimum_tls_version(&self, version: TlsVersion) -> Result<()> {
+        // `SSL_CTX_set_min_proto_version` is a C macro.
+        if unsafe {
+            openssl3::SSL_CTX_ctrl(
+                self.0.as_ptr(),
+                openssl3::SSL_CTRL_SET_MIN_PROTO_VERSION as i32,
+                version.into(),
+                ptr::null_mut(),
+            )
+        } == 1
+        {
+            Ok(())
+        } else {
+            Err((
+                pb::TLSConfigurationError::TLSCONFIGURATIONERROR_UNSUPPORTED_PROTOCOL_VERSION,
+                format!(
+                    "failed to set the minimum TLS version: {}",
+                    crate::ossl3::errstr()
+                ),
+            )
+                .into())
+        }
+    }
+
+    /// Defines the maximum TLS version to use.
+    fn set_maximum_tls_version(&self, version: TlsVersion) -> Result<()> {
+        // `SSL_CTX_set_max_proto_version` is a C macro.
+        if unsafe {
+            openssl3::SSL_CTX_ctrl(
+                self.0.as_ptr(),
+                openssl3::SSL_CTRL_SET_MAX_PROTO_VERSION as i32,
+                version.into(),
+                ptr::null_mut(),
+            )
+        } == 1
+        {
+            Ok(())
+        } else {
+            Err((
+                pb::TLSConfigurationError::TLSCONFIGURATIONERROR_UNSUPPORTED_PROTOCOL_VERSION,
+                format!(
+                    "failed to set the maximum TLS version: {}",
+                    crate::ossl3::errstr()
+                ),
+            )
+                .into())
+        }
+    }
+
+    /// Sets the minimum and the maximum TLS versions to use.
+    fn set_min_and_max_tls_version(&self, tls_options: &pb_api::TLSOptions) -> Result<()> {
+        let (min_version, max_version) =
+            tls::support::tls_options_get_min_max_tls_version(tls_options);
+        self.set_minimum_tls_version(min_version)?;
+        self.set_maximum_tls_version(max_version)
+    }
+
+    /// Initializes the trusted certificate store.
+    fn initialize_trusted_cert_store(&self) -> Result<()> {
+        let x509_store = NonNull::new(unsafe { openssl3::X509_STORE_new() }).ok_or((
+            pb::SystemError::SYSTEMERROR_MEMORY,
+            "failed to instantiate an X509_STORE",
+        ))?;
+
+        unsafe {
+            openssl3::SSL_CTX_set_cert_store(self.0.as_ptr(), x509_store.as_ptr());
+        }
+
+        Ok(())
+    }
+
+    /// Sets the trust parameter on the verification parameters object, depending
+    /// on the execution mode.
+    fn set_trust(&self, mode: Mode) -> Result<()> {
+        if unsafe {
+            openssl3::SSL_CTX_set_trust(
+                self.0.as_ptr(),
+                match mode {
+                    Mode::Client => openssl3::X509_TRUST_SSL_CLIENT,
+                    Mode::Server => openssl3::X509_TRUST_SSL_SERVER,
+                } as c_int,
+            )
+        } == 1
+        {
+            Ok(())
+        } else {
+            Err((
+                pb::SystemError::SYSTEMERROR_BACKEND,
+                format!("failed to set the trust parameter: {}", crate::ossl3::errstr()),
+            )
+                .into())
+        }
+    }
+
+    /// Sets the `SSL_MODE_RELEASE_BUFFERS` option.
+    ///
+    /// See <https://www.openssl.org/docs/man3.2/man3/SSL_CTX_set_mode.html#SSL_MODE_RELEASE_BUFFERS>
+    /// for more information.
+    fn set_mode_release_buffers(&self) {
+        // `SSL_CTX_set_mode` is a C macro.
+        unsafe {
+            openssl3::SSL_CTX_ctrl(
+                self.0.as_ptr(),
+                openssl3::SSL_CTRL_MODE as c_int,
+                openssl3::SSL_MODE_RELEASE_BUFFERS.into(),
+                ptr::null_mut(),
+            )
+        };
+    }
+
+    /// Sets the default parameters for a SSL context.
+    fn set_default_parameters(&self) -> Result<()> {
+        const DISABLED: c_int = 0;
+
+        unsafe {
+            openssl3::SSL_CTX_set_quiet_shutdown(self.0.as_ptr(), DISABLED);
+        }
+
+        self.disable_session_cache_mode();
+        self.set_mode_release_buffers();
+        self.initialize_trusted_cert_store()
+    }
+
+    /// Sets the list of available ciphers.
+    /// This function is only used for TLS 1.2.
+    /// Names will be converted to OpenSSL names using `OPENSSL_cipher_name`.
+    fn set_cipher_list<S>(&self, ciphers: impl IntoIterator<Item = S>) -> Result<()>
+    where
+        S: AsRef<str>,
+    {
+        let ciphersuites = tls::support::build_ciphersuites_list(
+            ciphers.into_iter().filter_map(crate::ossl3::cipher_name),
+            "!+@-",
+        )?;
+        let cstr = CString::new(ciphersuites).map_err(|e| {
+            (
+                pb::SystemError::SYSTEMERROR_MEMORY,
+                format!("failed to build a `CString`: {e}"),
+            )
+        })?;
+        if unsafe { openssl3::SSL_CTX_set_cipher_list(self.0.as_ptr(), cstr.as_ptr()) } == 1 {
+            Ok(())
+        } else {
+            Err((
+                pb::TLSConfigurationError::TLSCONFIGURATIONERROR_UNSUPPORTED_CIPHERSUITE,
+                format!("failed to set the cipher list: {}", crate::ossl3::errstr()),
+            )
+                .into())
+        }
+    }
+
+    /// Sets the list of available ciphers using the default list provided
+    /// by OpenSSL.
+    /// This function is only useful for TLS 1.2.
+    fn set_default_cipher_list(&self) -> Result<()> {
+        let cstr =
+            NonNull::new(unsafe { openssl3::OSSL_default_cipher_list() }.cast_mut()).ok_or((
+                pb::SystemError::SYSTEMERROR_BACKEND,
+                "`OSSL_default_cipher_list` returned NULL",
+            ))?;
+        if unsafe { openssl3::SSL_CTX_set_cipher_list(self.0.as_ptr(), cstr.as_ptr()) } == 1 {
+            Ok(())
+        } else {
+            Err((
+                pb::TLSConfigurationError::TLSCONFIGURATIONERROR_UNSUPPORTED_CIPHERSUITE,
+                format!("failed to set the cipher list: {}", crate::ossl3::errstr()),
+            )
+                .into())
+        }
+    }
+
+    /// Sets the list of available ciphersuites for TLS 1.3.
+    fn set_ciphersuites<S>(&self, ciphers: impl IntoIterator<Item = S>) -> Result<()>
+    where
+        S: AsRef<str>,
+    {
+        let control_string = tls::support::build_ciphersuites_list(ciphers, "!+@-")?;
+
+        let cstr = CString::new(control_string).map_err(|e| {
+            (
+                pb::SystemError::SYSTEMERROR_MEMORY,
+                format!("failed to build a `CString`: {e}"),
+            )
+        })?;
+        if unsafe { openssl3::SSL_CTX_set_ciphersuites(self.0.as_ptr(), cstr.as_ptr()) } == 1 {
+            Ok(())
+        } else {
+            Err((
+                pb::TLSConfigurationError::TLSCONFIGURATIONERROR_UNSUPPORTED_CIPHERSUITE,
+                format!("failed to set the ciphersuites: {}", crate::ossl3::errstr()),
+            )
+                .into())
+        }
+    }
+
+    /// Sets the list of available ciphersuites using the default list provided
+    /// by OpenSSL.
+    /// This function is only useful for TLS 1.3.
+    fn set_default_ciphersuites(&self) -> Result<()> {
+        let cstr = NonNull::new(unsafe { openssl3::OSSL_default_ciphersuites() }.cast_mut())
+            .ok_or((
+                pb::SystemError::SYSTEMERROR_BACKEND,
+                "`OSSL_default_ciphersuites` returned NULL",
+            ))?;
+        if unsafe { openssl3::SSL_CTX_set_ciphersuites(self.0.as_ptr(), cstr.as_ptr()) } == 1 {
+            Ok(())
+        } else {
+            Err((
+                pb::TLSConfigurationError::TLSCONFIGURATIONERROR_UNSUPPORTED_CIPHERSUITE,
+                format!("failed to set the ciphersuites: {}", crate::ossl3::errstr()),
+            )
+                .into())
+        }
+    }
+
+    /// Configures TLS 1.2.
+    fn configure_tls12(&self, tls12_config: Option<&pb_api::TLSv12Config>) -> Result<()> {
+        let Some(config) = tls12_config else {
+            return Ok(());
+        };
+        if config.ciphersuite.is_empty() {
+            self.set_default_cipher_list()?;
+        } else {
+            self.set_cipher_list(&config.ciphersuite)?;
+        }
+
+        Ok(())
+    }
+
+    /// Configures TLS 1.3.
+    fn configure_tls13(&self, tls13_config: Option<&pb_api::TLSv13Config>) -> Result<()> {
+        let Some(config) = tls13_config else {
+            return Ok(());
+        };
+
+        self.set_kes(&config.ke)?;
+
+        if config.ciphersuite.is_empty() {
+            self.set_default_ciphersuites()?;
+        } else {
+            self.set_ciphersuites(&config.ciphersuite)?;
+        }
+
+        Ok(())
+    }
+
+    /// Sets the KEs to an SSL context.
+    fn set_kes(&self, kes: &[impl AsRef<str>]) -> Result<()> {
+        if kes.is_empty() {
+            return Err((pb::KEMError::KEMERROR_INVALID, "no KE specified").into());
+        }
+
+        let list = CString::new(kes.iter().map(|s| s.as_ref()).collect::<Vec<_>>().join(":"))
+            .map_err(|e| {
+                (
+                    pb::SystemError::SYSTEMERROR_MEMORY,
+                    format!("failed to create the string list of KEs: {e}"),
+                )
+            })?;
+
+        // `SSL_CTX_set1_groups_list` is a C macro.
+        if unsafe {
+            openssl3::SSL_CTX_ctrl(
+                self.0.as_ptr(),
+                openssl3::SSL_CTRL_SET_GROUPS_LIST as i32,
+                0,
+                list.as_ptr().cast_mut().cast(),
+            )
+        } == 1
+        {
+            Ok(())
+        } else {
+            Err((pb::KEMError::KEMERROR_INVALID, crate::ossl3::errstr()).into())
+        }
+    }
+
+    /// Sets supported application protocols (ALPN).
+    fn set_alpn_protocols<S>(&self, protocols: impl IntoIterator<Item = S>) -> Result<()>
+    where
+        S: AsRef<str>,
+    {
+        let mut protos = String::new();
+        for proto in protocols.into_iter() {
+            let proto = proto.as_ref();
+            let x: u8 = proto.len().try_into().map_err(|_| {
+                (
+                    pb::ALPNError::ALPNERROR_LENGTH_ERROR,
+                    "ALPN length overflow",
+                )
+            })?;
+            if x == 0 {
+                return Err((
+                    pb::ALPNError::ALPNERROR_LENGTH_ERROR,
+                    "ALPN length erro: empty",
+                )
+                    .into());
+            }
+            if proto.contains(0x00_u8 as char) {
+                return Err((
+                    pb::ALPNError::ALPNERROR_INVALID_STRING,
+                    "string cannot contain null bytes",
+                )
+                    .into());
+            }
+            protos.push(x as char);
+            protos.push_str(proto);
+        }
+
+        let len: u32 = protos.len().try_into().map_err(|_| {
+            (
+                pb::SystemError::SYSTEMERROR_INTEGER_OVERFLOW,
+                "protos string is too large",
+            )
+        })?;
+        let cstr = CString::new(protos.as_bytes()).map_err(|e| {
+            (
+                pb::SystemError::SYSTEMERROR_MEMORY,
+                format!("failed to create a CString: {e}"),
+            )
+        })?;
+        if unsafe { openssl3::SSL_CTX_set_alpn_protos(self.0.as_ptr(), cstr.as_ptr().cast(), len) }
+            == 0
+        {
+            Ok(())
+        } else {
+            Err(pb::ALPNError::ALPNERROR_INVALID_STRING.into())
+        }
+    }
+
+    /// Sets the certificate to use when the remote peer requests an authentication.
+    /// This is used in server mode and in client mode when mTLS is enabled.
+    fn set_certificate(&self, certificate: NonNull<NativeX509Certificate>) -> Result<()> {
+        if unsafe { openssl3::SSL_CTX_use_certificate(self.0.as_ptr(), certificate.as_ptr()) } == 1
+        {
+            Ok(())
+        } else {
+            Err((
+                pb::CertificateError::CERTIFICATEERROR_UNSUPPORTED,
+                format!(
+                    "failed to use certificate for authentication: {}",
+                    crate::ossl3::errstr()
+                ),
+            )
+                .into())
+        }
+    }
+
+    /// Sets the private key to use when the remote peer is requesting an authentication.
+    /// This is used in server mode and in clinet mode when mTLS is enabled.
+    ///
+    /// This method also checks the consistency between the provided certificate
+    /// and the private key.
+    /// The certificate is provided using [`SslContext::set_certificate`].
+    fn set_private_key(&self, private_key: NonNull<NativePrivateKey>) -> Result<()> {
+        if unsafe { openssl3::SSL_CTX_use_PrivateKey(self.0.as_ptr(), private_key.as_ptr()) } != 1 {
+            return Err((
+                pb::PrivateKeyError::PRIVATEKEYERROR_UNSUPPORTED,
+                format!(
+                    "failed to use private key for authentication: {}",
+                    crate::ossl3::errstr()
+                ),
+            )
+                .into());
+        };
+
+        if unsafe { openssl3::SSL_CTX_check_private_key(self.0.as_ptr()) } == 1 {
+            Ok(())
+        } else {
+            Err((pb::TLSConfigurationError::TLSCONFIGURATIONERROR_PRIVATE_KEY_INCONSISTENT_WITH_CERTIFICATE,
+                format!("private key does not match certificate: {}", crate::ossl3::errstr())).into())
+        }
+    }
+
+    /// Appends a certificate to the certificate chain the peer is going to expose
+    /// to remote.
+    ///
+    /// This function takes a [`Pimpl`] as input since [`SSL_CTX_add_extra_chain_cert`]
+    /// takes the ownership of the `X509` object.
+    fn add_extra_chain_cert<'a, 'b>(
+        &self,
+        extra_certificate: Pimpl<'b, NativeX509Certificate>,
+    ) -> Result<()>
+    where
+        'a: 'b,
+    {
+        // `SSL_CTX_add_extra_chain_cert` is a C macro.
+        if unsafe {
+            openssl3::SSL_CTX_ctrl(
+                self.0.as_ptr(),
+                openssl3::SSL_CTRL_EXTRA_CHAIN_CERT as c_int,
+                0,
+                extra_certificate.as_nonnull().as_ptr().cast(),
+            )
+        } == 1
+        {
+            // [`SSL_CTX_add_extra_chain_cert`] takes the ownership of the given
+            // `X509` object.
+            extra_certificate.into_raw();
+            Ok(())
+        } else {
+            Err((
+                pb::CertificateError::CERTIFICATEERROR_UNSUPPORTED,
+                format!(
+                    "failed to add an extra certificate to the certificate chain: {}",
+                    crate::ossl3::errstr()
+                ),
+            )
+                .into())
+        }
+    }
+
+    /// Sets the X.509 identity to use.
+    /// If the client sets an X.509 identity, then it will expect a client
+    /// certificate request from the server, in order to establish a mutual
+    /// TLS tunnel (mTLS).
+    fn set_identity(
+        &self,
+        lib_ctx: &LibCtx<'_>,
+        identity: Option<&pb_api::X509Identity>,
+    ) -> Result<()> {
+        let Some(identity) = identity else {
+            return Ok(());
+        };
+        let (certificate_chain_format, data_source) = identity
+            .certificate
+            .as_ref()
+            .ok_or(pb::CertificateError::CERTIFICATEERROR_MALFORMED.into())
+            .and_then(tls::support::configuration_read_certificate)
+            .map_err(|e| e >> pb::TLSConfigurationError::TLSCONFIGURATIONERROR_INVALID)?;
+        let cert_chain_bio = crate::ossl3::BIO_from_buffer(&data_source)?;
+        let leaf_certificate = crate::ossl3::X509_from_BIO(
+            lib_ctx,
+            cert_chain_bio.as_nonnull(),
+            certificate_chain_format,
+        )?;
+        self.set_certificate(leaf_certificate.as_nonnull())?;
+
+        let (format, data_source) = identity
+            .private_key
+            .as_ref()
+            .ok_or(pb::PrivateKeyError::PRIVATEKEYERROR_MALFORMED.into())
+            .and_then(tls::support::configuration_read_private_key)
+            .map_err(|e| e >> pb::TLSConfigurationError::TLSCONFIGURATIONERROR_INVALID)?;
+        let bio = crate::ossl3::BIO_from_buffer(&data_source)?;
+        let private_key = crate::ossl3::EVP_PKEY_from_BIO(lib_ctx, bio.as_nonnull(), format)?;
+        self.set_private_key(private_key.as_nonnull())?;
+
+        while !crate::ossl3::is_BIO_eof(cert_chain_bio.as_nonnull()) {
+            let certificate_in_chain = crate::ossl3::X509_from_BIO(
+                lib_ctx,
+                cert_chain_bio.as_nonnull(),
+                certificate_chain_format,
+            )?;
+            self.add_extra_chain_cert(certificate_in_chain)?;
+        }
+
+        Ok(())
+    }
+
+    /// Imports the trusted certificates from the protobuf configuration to the
+    /// OpenSSL SSL context.
+    fn fill_certificate_trust_store(
+        &self,
+        lib_ctx: &LibCtx<'_>,
+        x509_verifier: Option<&pb_api::X509Verifier>,
+    ) -> Result<()> {
+        let Some(x509_verifier) = x509_verifier else {
+            return Ok(());
+        };
+
+        let store = NonNull::new(unsafe { openssl3::SSL_CTX_get_cert_store(self.0.as_ptr()) })
+            .ok_or((
+                pb::SystemError::SYSTEMERROR_MEMORY,
+                "SSL_CTX does not have a certificate store",
+            ))?;
+
+        for certificate in x509_verifier.trusted_cas.iter() {
+            let (format, data_source) = tls::support::configuration_read_certificate(certificate)?;
+            let bio = crate::ossl3::BIO_from_buffer(&data_source)?;
+
+            while !crate::ossl3::is_BIO_eof(bio.as_nonnull()) {
+                let x509 = crate::ossl3::X509_from_BIO(lib_ctx, bio.as_nonnull(), format)?;
+                unsafe {
+                    openssl3::X509_STORE_add_cert(store.as_ptr(), x509.as_nonnull().as_ptr())
+                };
+            }
+        }
+
+        Ok(())
+    }
+
+    /// Loads the OpenSSL system-default trust anchors into context store.
+    fn fill_certificate_trust_store_with_default_cas(
+        &self,
+        x509_verifier: Option<&pb_api::X509Verifier>,
+    ) -> Result<()> {
+        let Some(x509) = x509_verifier else {
+            return Ok(());
+        };
+
+        if x509.load_cas_from_default_verify_path
+            && unsafe { openssl3::SSL_CTX_set_default_verify_paths(self.0.as_ptr()) } != 1
+        {
+            return Err((
+                    pb::CertificateError::CERTIFICATEERROR_UNKNOWN,
+                    format!(
+                        "CAfile and CApath are NULL or the processing at one of the locations specified failed: {}",
+                        crate::ossl3::errstr()
+                    ),
+                    )
+                    .into());
+        }
+        Ok(())
+    }
+    /// Sets the verification mode.
+    ///
+    /// If a `X509Verifier` structure is present in the protobuf configuration,
+    /// then `SSL_VERIFY_PEER` is used in client mode, and `SSL_VERIFY_PEER | SSL_VERIFY_FAIL_IF_NO_PEER_CERT`
+    /// is used in server mode.
+    fn set_verify_mode(&self, verify_mode: VerifyMode) {
+        let flag = match verify_mode {
+            VerifyMode::None => openssl3::SSL_VERIFY_NONE,
+            VerifyMode::Peer => openssl3::SSL_VERIFY_PEER,
+            VerifyMode::Mutual => {
+                openssl3::SSL_VERIFY_PEER | openssl3::SSL_VERIFY_FAIL_IF_NO_PEER_CERT
+            }
+        };
+        unsafe {
+            openssl3::SSL_CTX_set_verify(self.0.as_ptr(), flag as i32, Some(verify_callback));
+        }
+    }
+}
+
+/// Instantiates a new SSL object from an SSL context.
+///
+/// `Pimpl` is passed here instead of the regular `NonNull` to enforce the lifetime
+/// of the resulting SSL object.
+fn ssl_context_new_ssl<'a, 'b>(
+    ssl_context: &Pimpl<'a, NativeSslCtx>,
+) -> Result<Pimpl<'b, NativeSsl>>
+where
+    'a: 'b,
+{
+    unsafe {
+        Pimpl::new(openssl3::SSL_new(ssl_context.as_nonnull().as_ptr()), |x| {
+            openssl3::SSL_free(x)
+        })
+    }
+    .ok_or_else(|| {
+        (
+            pb::SystemError::SYSTEMERROR_MEMORY,
+            format!("failed to instantiate a new SSL: {}", crate::ossl3::errstr()),
+        )
+            .into()
+    })
+}
+
+/// Determines the verify mode depending on the mode and the existence of a
+/// X509Verifier structure in the protobuf configuration.
+fn get_verify_mode_from_mode_and_x509_verifier(
+    mode: Mode,
+    x509_verifier: Option<&pb_api::X509Verifier>,
+) -> VerifyMode {
+    if x509_verifier.is_none() {
+        VerifyMode::None
+    } else if mode == Mode::Client {
+        VerifyMode::Peer
+    } else {
+        VerifyMode::Mutual
+    }
+}
+
+/// A boxed and pinned tunnel.
+pub(crate) type PinnedTunnel<'a> = Pin<Box<Tunnel<'a>>>;
+
+impl<'a> Context<'a> {
+    /// Instantiates a new [`Context`] from a [protobuf configuration](`pb_api::Configuration`)
+    /// and a top-level context.
+    pub(crate) fn try_from<'b>(
+        lib_ctx: &'a LibCtx<'static>,
+        configuration: &pb_api::Configuration,
+    ) -> Result<Self>
+    where
+        'b: 'a,
+    {
+        let (mode, tls_options) = tls::support::configuration_get_mode_and_options(configuration)?;
+        let ssl_ctx = new_ssl_context(lib_ctx, mode)?;
+        let ssl_ctx_wrapped = SslContext(ssl_ctx.as_nonnull());
+
+        ssl_ctx_wrapped.set_default_parameters()?;
+        ssl_ctx_wrapped.set_trust(mode)?;
+        ssl_ctx_wrapped.set_min_and_max_tls_version(tls_options)?;
+        ssl_ctx_wrapped.configure_tls12(tls_options.tls12.as_ref())?;
+        ssl_ctx_wrapped.configure_tls13(tls_options.tls13.as_ref())?;
+        ssl_ctx_wrapped.set_alpn_protocols(tls_options.alpn_protocols.iter())?;
+
+        let x509_verify_param = X509VerifyParam::try_from(&ssl_ctx)?;
+        x509_verify_param.set_default_parameters()?;
+
+        let x509_verifier = tls::support::tls_options_get_x509_verifier(tls_options)
+            .and_then(tls::support::x509_verifier_verify_emptiness)?;
+        x509_verify_param
+            .update_certificate_chain_validation_depth_from_x509_verifier(x509_verifier);
+
+        ssl_ctx_wrapped.set_identity(lib_ctx, tls_options.identity.as_ref())?;
+        ssl_ctx_wrapped.fill_certificate_trust_store(lib_ctx, x509_verifier)?;
+        ssl_ctx_wrapped.fill_certificate_trust_store_with_default_cas(x509_verifier)?;
+
+        let verify_mode = get_verify_mode_from_mode_and_x509_verifier(mode, x509_verifier);
+        ssl_ctx_wrapped.set_verify_mode(verify_mode);
+
+        let security_requirements = x509_verifier
+            .map(tls::TunnelSecurityRequirements::from)
+            .unwrap_or_default();
+
+        Ok(Self {
+            _lib_ctx: lib_ctx,
+            mode,
+            security_requirements,
+            ssl_ctx,
+        })
+    }
+
+    /// Instantiates a new SSL object.
+    pub(crate) fn new_ssl<'b>(&self) -> Result<Pimpl<'b, NativeSsl>>
+    where
+        'a: 'b,
+    {
+        let ssl = ssl_context_new_ssl(&self.ssl_ctx)?;
+        match self.mode {
+            Mode::Client => unsafe { openssl3::SSL_set_connect_state(ssl.as_nonnull().as_ptr()) },
+            Mode::Server => unsafe { openssl3::SSL_set_accept_state(ssl.as_nonnull().as_ptr()) },
+        };
+        Ok(ssl)
+    }
+
+    /// Returns the security requirements of the context.
+    pub(crate) fn security_requirements(&self) -> &tls::TunnelSecurityRequirements {
+        self.borrow()
+    }
+
+    /// Creates a new tunnel.
+    pub(crate) fn new_tunnel(
+        &self,
+        io: BoxedIO,
+        configuration: pb_api::TunnelConfiguration,
+    ) -> std::result::Result<PinnedTunnel<'_>, (crate::Error, BoxedIO)> {
+        TunnelBuilder {
+            ssl_ctx: self,
+            io,
+            configuration,
+        }
+        .build()
+    }
+}
+
+#[cfg(test)]
+mod test {
+    use super::*;
+
+    /// Returns the maximum depth for certificate chain validation.
+    fn ssl_context_get_verify_depth(ssl_ctx: NonNull<NativeSslCtx>) -> i32 {
+        unsafe { openssl3::SSL_CTX_get_verify_depth(ssl_ctx.as_ptr()) }
+    }
+
+    /// Tests [`new_ssl_context`] in client mode.
+    #[test]
+    fn test_new_ssl_context_client() {
+        let ctx = crate::Context::default();
+
+        new_ssl_context(&ctx, Mode::Client).unwrap();
+    }
+
+    /// Tests [`new_ssl_context`] in server mode.
+    #[test]
+    fn test_new_ssl_context_server() {
+        let ctx = crate::Context::default();
+
+        new_ssl_context(&ctx, Mode::Server).unwrap();
+    }
+
+    /// Tests [`SslContext::disable_session_cache_mode`].
+    #[test]
+    fn test_ssl_context_disable_session_cache_mode() {
+        let ctx = crate::Context::default();
+        let ssl_ctx = new_ssl_context(&ctx, Mode::Client).unwrap();
+        let ssl_ctx_wrapped = SslContext(ssl_ctx.as_nonnull());
+        ssl_ctx_wrapped.disable_session_cache_mode();
+
+        let result = unsafe {
+            // `SSL_CTX_get_session_cache_mode` is a C macro.
+            openssl3::SSL_CTX_ctrl(
+                ssl_ctx.as_nonnull().as_ptr(),
+                openssl3::SSL_CTRL_GET_SESS_CACHE_MODE as i32,
+                0,
+                ptr::null_mut(),
+            )
+        };
+
+        assert_eq!(result, openssl3::SSL_SESS_CACHE_OFF.into());
+    }
+
+    /// Tests [`SslContext::set_minimum_version`].
+    #[test]
+    fn test_ssl_context_set_minimum_version() {
+        let ctx = crate::Context::default();
+        let ssl_ctx = new_ssl_context(&ctx, Mode::Client).unwrap();
+        let ssl_ctx_wrapped = SslContext(ssl_ctx.as_nonnull());
+        let result = ssl_ctx_wrapped.set_minimum_tls_version(TlsVersion::Tls13);
+
+        let min_proto = unsafe {
+            // `SSL_CTX_get_min_proto_version` is a C macro.
+            openssl3::SSL_CTX_ctrl(
+                ssl_ctx.as_nonnull().as_ptr(),
+                openssl3::SSL_CTRL_GET_MIN_PROTO_VERSION as i32,
+                0,
+                ptr::null_mut(),
+            )
+        };
+
+        result.expect("fail to set minimum version for TLS protocol");
+        assert_eq!(min_proto, openssl3::TLS1_3_VERSION.into());
+    }
+
+    /// Tests [`SslContext::initialize_trusted_cert_store`].
+    #[test]
+    fn test_ssl_context_initialize_trusted_cert_store() {
+        let ctx = crate::Context::default();
+        let ssl_ctx = new_ssl_context(&ctx, Mode::Client).unwrap();
+        let ssl_ctx_wrapped = SslContext(ssl_ctx.as_nonnull());
+        let result_init = ssl_ctx_wrapped.initialize_trusted_cert_store();
+
+        let result = NonNull::new(unsafe {
+            openssl3::SSL_CTX_get_cert_store(ssl_ctx.as_nonnull().as_ptr())
+        });
+
+        result_init.expect("`SslContext::initialize_trusted_cert_store` failed");
+        result.expect("certificate store is NULL");
+    }
+
+    /// Tests [`SslContext::set_default_parameters`].
+    #[test]
+    fn test_ssl_context_set_default_parameters() {
+        let ctx = crate::Context::default();
+        let ssl_ctx = new_ssl_context(&ctx, Mode::Client).unwrap();
+        let ssl_ctx_wrapped = SslContext(ssl_ctx.as_nonnull());
+
+        let result = ssl_ctx_wrapped.set_default_parameters();
+
+        result.expect("`SslContext::set_default_parameters` failed");
+    }
+
+    /// Tests [`SslContext::set_ciphersuites`].
+
+    /// Tests [`SslContext::set_kes`].
+    #[test]
+    #[allow(non_snake_case)]
+    fn test_ssl_context_set_KEs() {
+        let ctx = crate::Context::default();
+        let ssl_ctx = new_ssl_context(&ctx, Mode::Client).unwrap();
+        let ssl_ctx_wrapped = SslContext(ssl_ctx.as_nonnull());
+
+        let result = ssl_ctx_wrapped.set_kes(&["X25519", "kyber768"]);
+
+        result.expect("`SslContext::set_kes` failed");
+    }
+
+    /// Tests [`SslContext::set_kes`] with invalid KE.
+    #[test]
+    #[allow(non_snake_case)]
+    fn test_ssl_context_set_KEs_invalid() {
+        let ctx = crate::Context::default();
+        let ssl_ctx = new_ssl_context(&ctx, Mode::Client).unwrap();
+        let ssl_ctx_wrapped = SslContext(ssl_ctx.as_nonnull());
+
+        let result = ssl_ctx_wrapped.set_kes(&["X25519", "kyber1337"]);
+
+        let err = result.expect_err("`SslContext::set_kes` succeed");
+        let e = err.iter().next().unwrap();
+        let msg = e.msg().unwrap();
+        assert!(msg.contains("group 'kyber1337' cannot be set"));
+    }
+
+    /// Tests [`SslContext::set_kes`] with no KE.
+    #[test]
+    #[allow(non_snake_case)]
+    fn test_ssl_context_set_KEs_empty() {
+        let ctx = crate::Context::default();
+        let ssl_ctx = new_ssl_context(&ctx, Mode::Client).unwrap();
+        let ssl_ctx_wrapped = SslContext(ssl_ctx.as_nonnull());
+
+        let empty: [&str; 0] = [];
+        let result = ssl_ctx_wrapped.set_kes(&empty);
+
+        let err = result.expect_err("`SslContext::set_kes` succeed");
+        let e = err.iter().next().unwrap();
+        let msg = e.msg().unwrap();
+        assert!(msg.contains("no KE specified"));
+    }
+
+    /// Tests [`SslContext::set_alpn_protocols`].
+    #[test]
+    fn test_ssl_context_set_alpn_protocols() {
+        let ctx = crate::Context::default();
+        let ssl_ctx = new_ssl_context(&ctx, Mode::Client).unwrap();
+        let ssl_ctx_wrapped = SslContext(ssl_ctx.as_nonnull());
+
+        let result = ssl_ctx_wrapped.set_alpn_protocols(["http/1.1", "h2", "h3", "h2c"]);
+
+        result.expect("`SslContext::set_alpn_protocols` failed");
+    }
+
+    /// Tests [`SslContext::set_alpn_protocols`] with a protocol containing a null byte.
+    #[test]
+    fn test_ssl_context_set_alpn_protocols_invalid_null_byte() {
+        let ctx = crate::Context::default();
+        let ssl_ctx = new_ssl_context(&ctx, Mode::Client).unwrap();
+        let ssl_ctx_wrapped = SslContext(ssl_ctx.as_nonnull());
+
+        let result = ssl_ctx_wrapped.set_alpn_protocols(["http/1.1", "h\x002"]);
+
+        let err = result.expect_err("`SslContext::set_alpn_protocols` succeed");
+        let e = err.iter().next().unwrap();
+        let msg = e.msg().unwrap();
+        assert!(msg.contains("string cannot contain null bytes"));
+    }
+
+    /// Tests [`SslContext::set_alpn_protocols`] with a protocol name of length > 255.
+    #[test]
+    fn test_ssl_context_set_alpn_protocols_invalid_too_long() {
+        let ctx = crate::Context::default();
+        let ssl_ctx = new_ssl_context(&ctx, Mode::Client).unwrap();
+        let ssl_ctx_wrapped = SslContext(ssl_ctx.as_nonnull());
+
+        let result = ssl_ctx_wrapped.set_alpn_protocols(["a".repeat(256)]);
+
+        let err = result.expect_err("`SslContext::set_alpn_protocols` succeed");
+        let e = err.iter().next().unwrap();
+        let msg = e.msg().unwrap();
+        assert!(msg.contains("ALPN length overflow"));
+    }
+
+    /// Tests [`SslContext::set_certificate`].
+    #[test]
+    fn test_ssl_context_set_certificate() {
+        let ctx = crate::Context::default();
+        let ssl_ctx = new_ssl_context(&ctx, Mode::Client).unwrap();
+        let ssl_ctx_wrapped = SslContext(ssl_ctx.as_nonnull());
+        let cert = crate::ossl3::test::get_certificate_from_testdata_file(
+            ctx.borrow(),
+            "testdata/falcon1024.cert.pem",
+            pb_api::ASN1EncodingFormat::ENCODING_FORMAT_PEM,
+        )
+        .unwrap();
+
+        let result = ssl_ctx_wrapped.set_certificate(cert.as_nonnull());
+
+        result.expect("`SslContext::set_certificate` failed");
+    }
+
+    /// Tests [`SslContext::set_private_key`].
+    #[test]
+    fn test_ssl_context_set_private_key() {
+        let ctx = crate::Context::default();
+        let ssl_ctx = new_ssl_context(&ctx, Mode::Client).unwrap();
+        let ssl_ctx_wrapped = SslContext(ssl_ctx.as_nonnull());
+        let cert = crate::ossl3::test::get_certificate_from_testdata_file(
+            ctx.borrow(),
+            "testdata/falcon1024.cert.pem",
+            pb_api::ASN1EncodingFormat::ENCODING_FORMAT_PEM,
+        )
+        .unwrap();
+        ssl_ctx_wrapped.set_certificate(cert.as_nonnull()).unwrap();
+        let private_key = crate::ossl3::test::get_private_key_from_testdata_file(
+            ctx.borrow(),
+            "testdata/falcon1024.key.pem",
+            pb_api::ASN1EncodingFormat::ENCODING_FORMAT_PEM,
+        )
+        .unwrap();
+
+        let result = ssl_ctx_wrapped.set_private_key(private_key.as_nonnull());
+
+        result.expect("`SslContext::set_private_key` failed");
+    }
+
+    /// Tests [`SslContext::set_private_key`] with inconsistent (certificate, private_key).
+    #[test]
+    fn test_ssl_context_set_private_key_inconsistent() {
+        let ctx = crate::Context::default();
+        let ssl_ctx = new_ssl_context(&ctx, Mode::Client).unwrap();
+        let ssl_ctx_wrapped = SslContext(ssl_ctx.as_nonnull());
+        let cert = crate::ossl3::test::get_certificate_from_testdata_file(
+            ctx.borrow(),
+            "testdata/falcon1024.cert.pem",
+            pb_api::ASN1EncodingFormat::ENCODING_FORMAT_PEM,
+        )
+        .unwrap();
+        ssl_ctx_wrapped.set_certificate(cert.as_nonnull()).unwrap();
+        let private_key = crate::ossl3::test::get_private_key_from_testdata_file(
+            ctx.borrow(),
+            "testdata/dilithium5.key.der",
+            pb_api::ASN1EncodingFormat::ENCODING_FORMAT_DER,
+        )
+        .unwrap();
+
+        let result = ssl_ctx_wrapped.set_private_key(private_key.as_nonnull());
+
+        let err = result.expect_err("`SslContext::set_private_key` succeed");
+        assert!(err.is(&errors!{pb::TLSConfigurationError::TLSCONFIGURATIONERROR_PRIVATE_KEY_INCONSISTENT_WITH_CERTIFICATE}));
+    }
+
+    /// Tests [`SslContext::add_extra_chain_cert`].
+    #[test]
+    fn test_ssl_context_add_extra_chain_cert() {
+        let ctx = crate::Context::default();
+        let ssl_ctx = new_ssl_context(&ctx, Mode::Client).unwrap();
+        let ssl_ctx_wrapped = SslContext(ssl_ctx.as_nonnull());
+        let cert = crate::ossl3::test::get_certificate_from_testdata_file(
+            ctx.borrow(),
+            "testdata/falcon1024.cert.pem",
+            pb_api::ASN1EncodingFormat::ENCODING_FORMAT_PEM,
+        )
+        .unwrap();
+        ssl_ctx_wrapped.set_certificate(cert.as_nonnull()).unwrap();
+
+        let result = ssl_ctx_wrapped.add_extra_chain_cert(cert);
+
+        result.expect("`SslContext::add_extra_chain_cert` failed");
+    }
+
+    /// Tests [`SslContext::set_identity`].
+    #[test]
+    fn test_ssl_context_set_identity() {
+        let ctx = crate::Context::default();
+        let ssl_ctx = new_ssl_context(&ctx, Mode::Client).unwrap();
+        let ssl_ctx_wrapped = SslContext(ssl_ctx.as_nonnull());
+        let identity = tls::support::test::create_x509_identity(
+            "testdata/falcon1024.cert.pem",
+            pb_api::ASN1EncodingFormat::ENCODING_FORMAT_PEM,
+            "testdata/falcon1024.key.pem",
+            pb_api::ASN1EncodingFormat::ENCODING_FORMAT_PEM,
+        );
+
+        let result = ssl_ctx_wrapped.set_identity(ctx.borrow(), Some(&identity));
+
+        result.expect("`SslContext::set_identity` failed");
+    }
+
+    /// Tests [`SslContext::set_identity`] with inconsistent certificate/key.
+    #[test]
+    fn test_ssl_context_set_identity_inconsistent() {
+        let ctx = crate::Context::default();
+        let ssl_ctx = new_ssl_context(&ctx, Mode::Client).unwrap();
+        let ssl_ctx_wrapped = SslContext(ssl_ctx.as_nonnull());
+        let identity = tls::support::test::create_x509_identity(
+            "testdata/falcon1024.cert.pem",
+            pb_api::ASN1EncodingFormat::ENCODING_FORMAT_PEM,
+            "testdata/dilithium5.key.der",
+            pb_api::ASN1EncodingFormat::ENCODING_FORMAT_DER,
+        );
+
+        let result = ssl_ctx_wrapped.set_identity(ctx.borrow(), Some(&identity));
+
+        let err = result.expect_err("`SslContext::set_identity` succeed");
+        assert!(err.is(&errors!{pb::TLSConfigurationError::TLSCONFIGURATIONERROR_PRIVATE_KEY_INCONSISTENT_WITH_CERTIFICATE}));
+    }
+
+    /// Tests [`SslContext::fill_certificate_trust_store`].
+    #[test]
+    fn test_ssl_context_fill_certificate_trust_store() {
+        let ctx = crate::Context::default();
+        let ssl_ctx = new_ssl_context(&ctx, Mode::Client).unwrap();
+        let ssl_ctx_wrapped = SslContext(ssl_ctx.as_nonnull());
+        let x509_verifier = tls::support::test::create_x509_verifier(
+            [(
+                "testdata/etc_ssl_cert.pem",
+                pb_api::ASN1EncodingFormat::ENCODING_FORMAT_PEM,
+            )],
+            false,
+            4u32,
+            false,
+        );
+
+        let result =
+            ssl_ctx_wrapped.fill_certificate_trust_store(ctx.borrow(), Some(&x509_verifier));
+
+        result.expect("`SslContext::fill_certificate_trust_store` failed");
+    }
+
+    /// Tests [`SslContext::fill_certificate_trust_store_with_default_cas`].
+    #[test]
+    fn test_ssl_context_fill_certificate_trust_store_with_default_cas() {
+        let ctx = crate::Context::default();
+        let ssl_ctx = new_ssl_context(&ctx, Mode::Client).unwrap();
+        let ssl_ctx_wrapped = SslContext(ssl_ctx.as_nonnull());
+        let x509_verifier = tls::support::test::create_x509_verifier(
+            [("", pb_api::ASN1EncodingFormat::ENCODING_FORMAT_PEM)],
+            false,
+            0u32,
+            true,
+        );
+
+        let result =
+            ssl_ctx_wrapped.fill_certificate_trust_store_with_default_cas(Some(&x509_verifier));
+
+        result.expect("`SslContext::fill_certificate_trust_store_with_default_ca` failed");
+    }
+
+    /// Tests [`SslContext::fill_certificate_trust_store`] with no X509Verifier.
+    #[test]
+    fn test_ssl_context_fill_certificate_trust_store_no_x509_verifier() {
+        let ctx = crate::Context::default();
+        let ssl_ctx = new_ssl_context(&ctx, Mode::Client).unwrap();
+        let ssl_ctx_wrapped = SslContext(ssl_ctx.as_nonnull());
+
+        let result = ssl_ctx_wrapped.fill_certificate_trust_store(ctx.borrow(), None);
+
+        result.expect("`SslContext::fill_certificate_trust_store` failed");
+    }
+
+    /// Tests [`SslContext::fill_certificate_trust_store`] with an invalid
+    /// certificate in the middle of the list.
+    #[test]
+    fn test_ssl_context_fill_certificate_trust_store_invalid() {
+        let ctx = crate::Context::default();
+        let ssl_ctx = new_ssl_context(&ctx, Mode::Client).unwrap();
+        let ssl_ctx_wrapped = SslContext(ssl_ctx.as_nonnull());
+        let x509_verifier = tls::support::test::create_x509_verifier(
+            [(
+                "testdata/etc_ssl_cert_invalid.pem",
+                pb_api::ASN1EncodingFormat::ENCODING_FORMAT_PEM,
+            )],
+            false,
+            4u32,
+            false,
+        );
+
+        let result =
+            ssl_ctx_wrapped.fill_certificate_trust_store(ctx.borrow(), Some(&x509_verifier));
+
+        let err = result.expect_err("`SslContext::fill_certificate_trust_store` succeed");
+        assert!(err.is(&errors! {pb::CertificateError::CERTIFICATEERROR_MALFORMED}));
+    }
+
+    /// Tests [`get_verify_mode_from_mode_and_x509_verifier`] in client mode
+    /// with an X509 verifier.
+    #[test]
+    fn test_get_verify_mode_from_mode_and_x509_verifier_client() {
+        let x509_verifier = tls::support::test::create_x509_verifier(
+            [(
+                "testdata/etc_ssl_cert.pem",
+                pb_api::ASN1EncodingFormat::ENCODING_FORMAT_PEM,
+            )],
+            false,
+            4u32,
+            false,
+        );
+
+        let result =
+            get_verify_mode_from_mode_and_x509_verifier(Mode::Client, Some(&x509_verifier));
+
+        assert_eq!(result, VerifyMode::Peer);
+    }
+
+    /// Tests [`get_verify_mode_from_mode_and_x509_verifier`] in client mode
+    /// with an no X509 verifier.
+    #[test]
+    fn test_get_verify_mode_from_mode_and_x509_verifier_client_no_verifier() {
+        let result = get_verify_mode_from_mode_and_x509_verifier(Mode::Client, None);
+
+        assert_eq!(result, VerifyMode::None);
+    }
+
+    /// Tests [`get_verify_mode_from_mode_and_x509_verifier`] in server mode
+    /// with no X509 verifier.
+    #[test]
+    fn test_get_verify_mode_from_mode_and_x509_verifier_server_no_verifier() {
+        let result = get_verify_mode_from_mode_and_x509_verifier(Mode::Server, None);
+
+        assert_eq!(result, VerifyMode::None);
+    }
+
+    /// Tests [`get_verify_mode_from_mode_and_x509_verifier`] in server mode
+    /// with an X509 verifier (mTLS).
+    #[allow(non_snake_case)]
+    #[test]
+    fn test_get_verify_mode_from_mode_and_x509_verifier_server_mTLS() {
+        let x509_verifier = tls::support::test::create_x509_verifier(
+            [(
+                "testdata/etc_ssl_cert.pem",
+                pb_api::ASN1EncodingFormat::ENCODING_FORMAT_PEM,
+            )],
+            false,
+            4u32,
+            false,
+        );
+
+        let result =
+            get_verify_mode_from_mode_and_x509_verifier(Mode::Server, Some(&x509_verifier));
+
+        assert_eq!(result, VerifyMode::Mutual);
+    }
+
+    /// Tests [`ssl_context_new_ssl`].
+    #[test]
+    fn test_ssl_context_new_ssl() {
+        let ctx = crate::Context::default();
+        let ssl_ctx = new_ssl_context(&ctx, Mode::Client).unwrap();
+
+        let result = ssl_context_new_ssl(&ssl_ctx);
+
+        result.expect("`ssl_context_new_ssl` failed");
+    }
+
+    /// Tests [`TryFrom`] for [`Context`].
+    #[test]
+    fn test_context_try_from() {
+        let ctx = crate::Context::default();
+        let configuration =
+            protobuf::text_format::parse_from_str::<pb_api::Configuration>(&format!(
+                r#"
+                impl: IMPL_OPENSSL3_OQS_PROVIDER
+                client <
+                    tls <
+                        common_options <
+                            tls13 <
+                                ke: "X25519"
+                                ke: "kyber768"
+                            >
+                            x509_verifier <
+                                trusted_cas <
+                                    static <
+                                        data <
+                                            filename: "{etc_ssl_cert_pem}"
+                                        >
+                                        format: ENCODING_FORMAT_PEM
+                                    >
+                                >
+                                max_verify_depth: 42
+                                load_cas_from_default_verify_path: false
+                            >
+                            identity <
+                                certificate <
+                                    static <
+                                        data <
+                                            filename: "{certificate_file}"
+                                        >
+                                        format: ENCODING_FORMAT_PEM
+                                    >
+                                >
+                                private_key <
+                                    static <
+                                        data <
+                                            filename: "{private_key_file}"
+                                        >
+                                        format: ENCODING_FORMAT_PEM
+                                    >
+                                >
+                            >
+                            alpn_protocols: "http/1.1"
+                        >
+                    >
+                >
+            "#,
+                etc_ssl_cert_pem =
+                    crate::test::resolve_runfile("testdata/etc_ssl_cert.pem"),
+                certificate_file =
+                    crate::test::resolve_runfile("testdata/falcon1024.cert.pem"),
+                private_key_file =
+                    crate::test::resolve_runfile("testdata/falcon1024.key.pem"),
+            ))
+            .unwrap();
+
+        let result = Context::try_from(&ctx, &configuration);
+
+        let context = result.expect("`try_from` failed");
+        assert_eq!(
+            ssl_context_get_verify_depth(context.ssl_ctx.as_nonnull()),
+            42
+        );
+    }
+}
+
+// ######### Inlining bio_method.rs ############ ///
+
+// Copyright (c) SandboxAQ. All rights reserved.
+// SPDX-License-Identifier: AGPL-3.0-only
+
+// Implementation of the Sandwich BIO method.
+
+use std::ffi::c_char;
+
+use crate::io::error::IntoIOError;
+
+use crate::tunnel::IO;
+
+use std::io::Read;
+use std::io::Write;
+
+
+/// A wrapper around a BIO.
+struct Bio(NonNull<NativeBio>);
+
+impl std::fmt::Debug for Bio {
+    fn fmt(&self, f: &mut std::fmt::Formatter) -> std::fmt::Result {
+        write!(f, "SandwichOpenSSL3BIO({:p})", self.0.as_ptr())
+    }
+}
+
+impl Bio {
+    /// Clears the BIO retry flag.
+    fn clear_retry_flag(&self) {
+        self.clear_flags((openssl3::BIO_FLAGS_RWS | openssl3::BIO_FLAGS_SHOULD_RETRY) as c_int);
+    }
+
+    /// Sets the 'retry read' flag.
+    fn set_retry_read_flag(&self) {
+        self.set_flags((openssl3::BIO_FLAGS_READ | openssl3::BIO_FLAGS_SHOULD_RETRY) as c_int);
+    }
+
+    /// Sets the 'retry write' flag.
+    fn set_retry_write_flag(&self) {
+        self.set_flags((openssl3::BIO_FLAGS_WRITE | openssl3::BIO_FLAGS_SHOULD_RETRY) as c_int);
+    }
+
+    /// Declares the BIO as closed.
+    fn declare_closed(&self) {
+        // `BIO_set_close` is a C macro.
+        unsafe {
+            openssl3::BIO_ctrl(
+                self.0.as_ptr(),
+                openssl3::BIO_CTRL_SET_CLOSE as c_int,
+                1,
+                ptr::null_mut(),
+            )
+        };
+    }
+
+    /// Clears flags.
+    fn clear_flags(&self, flags: impl Into<c_int>) {
+        unsafe { openssl3::BIO_clear_flags(self.0.as_ptr(), flags.into()) };
+    }
+
+    /// Sets flags.
+    fn set_flags(&self, flags: impl Into<c_int>) {
+        unsafe { openssl3::BIO_set_flags(self.0.as_ptr(), flags.into()) };
+    }
+
+    /// Returns the tunnel attached to the BIO.
+    fn get_tunnel<'a>(&self) -> Option<&'a mut Tunnel<'a>> {
+        NonNull::new(unsafe { openssl3::BIO_get_data(self.0.as_ptr()) }.cast::<Tunnel<'a>>())
+            .map(|mut p| unsafe { p.as_mut() })
+    }
+
+    /// Returns the SSL object attached to the BIO.
+    fn get_ssl(&self) -> std::result::Result<NonNull<NativeSsl>, pb::IOError> {
+        let mut ssl = ptr::null_mut::<NativeSsl>();
+        if unsafe {
+            // `BIO_get_ssl` is a C macro.
+            openssl3::BIO_ctrl(
+                self.0.as_ptr(),
+                openssl3::BIO_C_GET_SSL as c_int,
+                0,
+                (&mut ssl as *mut *mut NativeSsl).cast(),
+            )
+        } == 1
+        {
+            Ok(unsafe { NonNull::new_unchecked(ssl) })
+        } else {
+            Err(pb::IOError::IOERROR_SYSTEM_ERROR)
+        }
+    }
+
+    /// Synchronizes the SSL state with the tunnel state.
+    fn synchronize_states(&self, tun: &'_ mut Tunnel<'_>) {
+        if tun.state != pb::State::STATE_HANDSHAKE_DONE {
+            if let Ok(ssl) = self.get_ssl() {
+                debug_assert!(ssl == tun.ssl.as_nonnull());
+                if unsafe { openssl3::SSL_get_state(ssl.as_ptr()) }
+                    == openssl3::OSSL_HANDSHAKE_STATE_TLS_ST_OK
+                {
+                    tun.state = pb::State::STATE_HANDSHAKE_DONE;
+                }
+            }
+        }
+    }
+
+    /// Reads data from the BIO.
+    fn read(&self, buffer: &mut [u8]) -> std::result::Result<usize, pb::IOError> {
+        let tun = self.get_tunnel().ok_or(pb::IOError::IOERROR_SYSTEM_ERROR)?;
+        self.synchronize_states(tun);
+        tun.io.set_state(tun.state);
+        tun.io.read(buffer).map_err(|e| e.into_io_error())
+    }
+
+    /// Writes data to the BIO.
+    fn write(&self, buffer: &[u8]) -> std::result::Result<usize, pb::IOError> {
+        let tun = self.get_tunnel().ok_or(pb::IOError::IOERROR_SYSTEM_ERROR)?;
+        self.synchronize_states(tun);
+        tun.io.set_state(tun.state);
+        tun.io.write(buffer).map_err(|e| e.into_io_error())
+    }
+
+    /// Flushes data.
+    fn flush(&self) -> std::result::Result<(), pb::IOError> {
+        let tun = self.get_tunnel().ok_or(pb::IOError::IOERROR_SYSTEM_ERROR)?;
+        (tun.io).flush().map_err(|e| e.into_io_error())
+    }
+}
+
+/// Reflects an IO error in the BIO flags.
+///
+/// When an IO interface raises an error, this function sets the appropriate
+/// flags to the BIO state depending on the error.
+fn bio_reflect_io_error(
+    error: pb::IOError,
+    on_retry: impl FnOnce() -> c_int,
+    on_close: impl FnOnce() -> c_int,
+    default_return_value: impl Into<c_int>,
+) -> c_int {
+    match error {
+        pb::IOError::IOERROR_IN_PROGRESS | pb::IOError::IOERROR_WOULD_BLOCK => on_retry(),
+        pb::IOError::IOERROR_CLOSED | pb::IOError::IOERROR_REFUSED => on_close(),
+        _ => default_return_value.into(),
+    }
+}
+
+/// BIO write callback.
+unsafe extern "C" fn bio_write(
+    bio: *mut NativeBio,
+    data: *const c_char,
+    len: usize,
+    written: *mut usize,
+) -> c_int {
+    let bio = Bio(NonNull::new_unchecked(bio));
+    bio.clear_retry_flag();
+    match bio.write(std::slice::from_raw_parts(data.cast(), len)) {
+        Ok(n) => {
+            *written = n;
+            1
+        }
+        Err(e) => bio_reflect_io_error(
+            e,
+            || {
+                bio.set_retry_write_flag();
+                -1
+            },
+            || {
+                bio.declare_closed();
+                -1
+            },
+            -1,
+        ),
+    }
+}
+
+/// BIO read callback.
+unsafe extern "C" fn bio_read(
+    bio: *mut NativeBio,
+    data: *mut c_char,
+    len: usize,
+    written: *mut usize,
+) -> c_int {
+    let bio = Bio(NonNull::new_unchecked(bio));
+    bio.clear_retry_flag();
+    match bio.read(std::slice::from_raw_parts_mut(data.cast(), len)) {
+        Ok(n) => {
+            *written = n;
+            1
+        }
+        Err(e) => bio_reflect_io_error(
+            e,
+            || {
+                bio.set_retry_read_flag();
+                -1
+            },
+            || {
+                bio.declare_closed();
+                -1
+            },
+            -1,
+        ),
+    }
+}
+
+/// BIO control callback.
+unsafe extern "C" fn bio_ctrl(
+    bio: *mut NativeBio,
+    cmd: c_int,
+    larg: i64,
+    _pargs: *mut c_void,
+) -> i64 {
+    match cmd as u32 {
+        openssl3::BIO_CTRL_SET_CLOSE => {
+            openssl3::BIO_set_shutdown(bio, larg as i32);
+            1
+        }
+        openssl3::BIO_CTRL_GET_CLOSE => openssl3::BIO_get_shutdown(bio) as i64,
+        openssl3::BIO_CTRL_FLUSH => {
+            if Bio(NonNull::new_unchecked(bio)).flush().is_err() {
+                0
+            } else {
+                1
+            }
+        }
+        _ => 0,
+    }
+}
+
+/// BIO create callback (never used).
+unsafe extern "C" fn bio_create(_bio: *mut openssl3::bio_st) -> c_int {
+    1
+}
+
+/// BIO destroy callback (never used).
+unsafe extern "C" fn bio_destroy(_bio: *mut NativeBio) -> c_int {
+    1
+}
+
+/// Static BIO method.
+pub(super) const BIO_METH_OBJECT: openssl3::bio_method_st = openssl3::bio_method_st {
+    type_: openssl3::BIO_TYPE_SOCKET as i32,
+    name: ptr::null_mut(),
+    bwrite: Some(bio_write),
+    bwrite_old: None,
+    bread: Some(bio_read),
+    bread_old: None,
+    bputs: None,
+    bgets: None,
+    ctrl: Some(bio_ctrl),
+    create: Some(bio_create),
+    destroy: Some(bio_destroy),
+    callback_ctrl: None,
+    brecvmmsg: None,
+    bsendmmsg: None,
+};
+
+pub(super) const BIO_METHOD: NonNull<openssl3::BIO_METHOD> =
+    unsafe { NonNull::new_unchecked((&BIO_METH_OBJECT as *const openssl3::BIO_METHOD).cast_mut()) };
+
+#[cfg(test)]
+mod test {
+    use super::*;
+    use crate::support::Pimpl;
+
+    /// Creates a new BIO.
+    fn new_bio(meth: Option<NonNull<openssl3::BIO_METHOD>>) -> Pimpl<'static, NativeBio> {
+        unsafe {
+            Pimpl::new(
+                openssl3::BIO_new(
+                    meth.map(|p| p.as_ptr().cast_const())
+                        .unwrap_or(openssl3::BIO_s_mem()),
+                ),
+                |x| openssl3::BIO_free_all(x),
+            )
+        }
+        .unwrap()
+    }
+
+    /// Returns a couple of bool that indicates if the read and write flags
+    /// are respectively set.
+    fn get_read_write_flags(bio: NonNull<NativeBio>) -> (bool, bool) {
+        (
+            unsafe {
+                // `BIO_should_read` is a C macro: `BIO_test_flags(ptr, BIO_FLAGS_READ)`.
+                openssl3::BIO_test_flags(bio.as_ptr(), openssl3::BIO_FLAGS_READ as c_int)
+            } == openssl3::BIO_FLAGS_READ as c_int,
+            unsafe {
+                // `BIO_should_write` is a C macro: `BIO_test_flags(ptr, BIO_FLAGS_WRITE)`
+                openssl3::BIO_test_flags(bio.as_ptr(), openssl3::BIO_FLAGS_WRITE as c_int)
+            } == openssl3::BIO_FLAGS_WRITE as c_int,
+        )
+    }
+
+    /// Declares a BIO as open (opposite to close).
+    fn set_open(bio: NonNull<NativeBio>) {
+        unsafe {
+            // `BIO_set_close` is a C macro.
+            openssl3::BIO_ctrl(
+                bio.as_ptr(),
+                openssl3::BIO_CTRL_SET_CLOSE as c_int,
+                0,
+                ptr::null_mut(),
+            )
+        };
+    }
+
+    /// Returns the closed state of a BIO.
+    fn get_close_state(bio: NonNull<NativeBio>) -> bool {
+        (unsafe {
+            // `BIO_get_close` is a C macro.
+            openssl3::BIO_ctrl(
+                bio.as_ptr(),
+                openssl3::BIO_CTRL_GET_CLOSE as c_int,
+                0,
+                ptr::null_mut(),
+            )
+        }) == 1
+    }
+
+    /// Tests [`Bio::clear_retry_flag`].
+    #[test]
+    fn test_clear_retry_flag() {
+        let bio = new_bio(None);
+        let bio_wrapped = Bio(bio.as_nonnull());
+        bio_wrapped.set_retry_read_flag();
+        bio_wrapped.set_retry_write_flag();
+        let flags_before = get_read_write_flags(bio.as_nonnull());
+        bio_wrapped.clear_retry_flag();
+
+        let result = get_read_write_flags(bio.as_nonnull());
+
+        assert_eq!((flags_before, result), ((true, true), (false, false)));
+    }
+
+    /// Tests [`Bio::set_retry_read_flag`].
+    #[test]
+    fn test_set_retry_read_flag() {
+        let bio = new_bio(None);
+        let bio_wrapped = Bio(bio.as_nonnull());
+        bio_wrapped.set_retry_read_flag();
+
+        let result = get_read_write_flags(bio.as_nonnull());
+
+        assert_eq!(result, (true, false));
+    }
+
+    /// Tests [`Bio::set_retry_read_flag`].
+    #[test]
+    fn test_set_retry_write_flag() {
+        let bio = new_bio(None);
+        let bio_wrapped = Bio(bio.as_nonnull());
+        bio_wrapped.set_retry_write_flag();
+
+        let result = get_read_write_flags(bio.as_nonnull());
+
+        assert_eq!(result, (false, true));
+    }
+
+    /// Tests [`Bio::declare_closed`].
+    #[test]
+    fn test_declare_closed() {
+        let bio = new_bio(None);
+        set_open(bio.as_nonnull());
+        let close_before = get_close_state(bio.as_nonnull());
+        let bio_wrapped = Bio(bio.as_nonnull());
+        bio_wrapped.declare_closed();
+
+        let result = get_close_state(bio.as_nonnull());
+
+        assert_eq!((close_before, result), (false, true));
+    }
 }
